src/program_proof/mvcc/txnmgr_activate_gc.v
@@ -1,0 +1,89 @@
+From Perennial.program_proof.mvcc Require Import
+     txn_prelude txnmgr_repr txnmgr_get_min_active_tid
+     index_proof.
+
+Section program.
+Context `{!heapGS Σ, !mvcc_ghostG Σ}.
+
+(*****************************************************************)
+(* func (txnMgr *TxnMgr) gc()                                    *)
+(*****************************************************************)
+Theorem wp_txnMgr__gc txnmgr γ :
+  is_txnmgr txnmgr γ -∗
+  {{{ True }}}
+    TxnMgr__gc #txnmgr
+  {{{ RET #(); True }}}.
+Proof.
+  iIntros "#Htxnmgr" (Φ) "!> _ HΦ".
+  wp_call.
+
+  (***********************************************************)
+  (* tidMin := txnMgr.getMinActiveTID()                      *)
+  (* if tidMin < config.TID_SENTINEL {                       *)
+  (*     txnMgr.idx.DoGC(tidMin)                             *)
+  (* }                                                       *)
+  (***********************************************************)
+  wp_apply (wp_txnMgr__getMinActiveTID with "Htxnmgr").
+  iIntros (tid) "#Hminlb".
+  wp_pures.
+  iNamed "Htxnmgr".
+  wp_if_destruct.
+  { (* Actually do the GC. *)
+    (*
+     * The loop condition is for performance, not correctness, so it's
+     * ignored in the proof.
+     *)
+    wp_loadField.
+    wp_apply (wp_index__DoGC with "HidxRI Hminlb").
+    wp_pures.
+    by iApply "HΦ".
+  }
+  (* Do nothing as no active txns. *)
+  by iApply "HΦ".
+Qed.
+
+(* TODO: Move this to the right place. *)
+Theorem wp_Sleep (t : u64) :
+  {{{ True }}}
+    Sleep #t
+  {{{ RET #(); True }}}.
+Admitted.
+
+(*****************************************************************)
+(* func (txnMgr *TxnMgr) ActivateGC()                            *)
+(*****************************************************************)
+Theorem wp_txnMgr__ActivateGC txnmgr γ :
+  is_txnmgr txnmgr γ -∗
+  {{{ True }}}
+    TxnMgr__ActivateGC #txnmgr
+  {{{ RET #(); True }}}.
+Proof.
+  iIntros "#Htxnmgr" (Φ) "!> _ HΦ".
+  wp_call.
+
+  (***********************************************************)
+  (* go func() {                                             *)
+  (*     for {                                               *)
+  (*         txnMgr.gc()                                     *)
+  (*         grove_ffi.Sleep(uint64(100) * uint64(1000000))  *)
+  (*     }                                                   *)
+  (* }()                                                     *)
+  (***********************************************************)
+  wp_apply wp_fork.
+  { (* Forked process. *)
+    wp_pures.
+    wp_apply (wp_forBreak (λ _, True)%I); last done.
+    clear Φ.
+    iIntros (Φ) "!> _ HΦ".
+    wp_pures.
+    wp_apply (wp_txnMgr__gc with "Htxnmgr").
+    wp_pures.
+    wp_apply wp_Sleep.
+    wp_pures.
+    by iApply "HΦ".
+  }
+  wp_pures.
+  by iApply "HΦ".
+Qed.
+
+End program.
